tests/lean/run/grind_eq_pattern.lean
@@ -1,4 +1,17 @@
+%reset_grind_attrs
+
+/--
+info: [grind.ematch.pattern] List.append_ne_nil_of_left_ne_nil: [@HAppend.hAppend ? ? ? ? #2 #0]
+-/
+#guard_msgs (info) in
+set_option trace.grind.ematch.pattern true in
 attribute [grind] List.append_ne_nil_of_left_ne_nil
+
+/--
+info: [grind.ematch.pattern] List.append_ne_nil_of_right_ne_nil: [@HAppend.hAppend ? ? ? ? #1 #2]
+-/
+#guard_msgs (info) in
+set_option trace.grind.ematch.pattern true in
 attribute [grind] List.append_ne_nil_of_right_ne_nil
 /--
 info: [grind.ematch.pattern] List.getLast?_eq_some_iff: [@List.getLast? #2 #1, @some ? #0]
@@ -13,7 +26,6 @@ info: [grind.assert] xs.getLast? = b?
 [grind.assert] xs = []
 [grind.assert] (xs.getLast? = some 10) = ∃ ys, xs = ys ++ [10]
 [grind.assert] xs = w ++ [10]
-[grind.assert] ¬w = [] → ¬w ++ [10] = []
 [grind.assert] ¬w ++ [10] = []
 -/
 #guard_msgs (info) in
